updates

Veritas.Verifier.Correctness.fst
@@ -28,43 +28,33 @@ module TL = Veritas.Verifier.TSLog
 //Allow the solver to invert inductive definitions at most once (ifuel)
 #push-options "--max_fuel 1 --max_ifuel 1 --initial_fuel 1 --initial_ifuel 1"
 
-(* 
- * an indexed version of time sequence where we track the source verifier thread 
- * for every log entry 
- *)
-let time_seq_idx (gl: VG.hash_verifiable_log): TL.hash_verifiable_log (S.length gl) =
-  admit()
-  //interleaved_idx_seq gl (time_seq_ctor gl)
-
 (* state ops of all vlogs of all verifier threads *)
 let to_state_op_gvlog (gl: g_vlog) =
   map to_state_op_vlog gl
 
-let lemma_time_seq_rw_consistent (#n:pos) 
-  (itsl: TL.hash_verifiable_log n{~ (rw_consistent (to_state_op_vlog (project_seq itsl)))})
-  : hash_collision_gen = 
-  let tsl = project_seq itsl in  
-  let tsle = time_seq_ext itsl in
-  assert(to_vlog tsle = tsl);
-
-  (* provided: the sequence of state ops is not rw-consistent *)
-  let ts_ops = to_state_op_vlog tsl in
-  assert(~ (rw_consistent ts_ops));
-
-  (* if time seq log is evict add consistent, the underlying state ops is rw-consistent *)
-  (* a contradiction *)
-  if E.is_eac_log tsle then (
-    lemma_eac_implies_rw_consistent tsle;
-    assert(rw_consistent ts_ops);
-
-    (* any return value *)
-    SingleHashCollision (Collision (DVal Null) (DVal Null)) 
-  )
-  else 
-    lemma_non_eac_time_seq_implies_hash_collision itsl
-
 let lemma_vlog_interleave_implies_state_ops_interleave (l: vlog) (gl: g_vlog{interleave l gl}):
   Lemma (interleave (to_state_op_vlog l) (to_state_op_gvlog gl)) = admit()
+
+let lemma_time_seq_rw_consistent  
+  (itsl: TL.hash_verifiable_log {~ (rw_consistent (state_ops itsl))})
+  : hash_collision_gen = 
+  let tsl = i_seq itsl in  
+  let ts_ops = to_state_op_vlog tsl in
+  
+  //assert(~ (rw_consistent ts_ops));
+
+  if TL.is_eac itsl then (
+    // ts log is eac implies state ops in that sequence are rw-consistent
+    TL.lemma_eac_implies_state_ops_rw_consistent itsl;
+
+    // ... which is a contradiction
+    //assert(rw_consistent ts_ops);
+
+    (* any return value *)
+    SingleHashCollision (Collision (DVal Null) (DVal Null))
+  )
+  else
+    lemma_non_eac_time_seq_implies_hash_collision itsl
 
 (* final verifier correctness theorem *)
 let lemma_verifier_correct (gl: VG.hash_verifiable_log { ~ (seq_consistent (to_state_op_gvlog gl))}):
@@ -73,26 +63,23 @@ let lemma_verifier_correct (gl: VG.hash_verifiable_log { ~ (seq_consistent (to_s
   let g_ops = to_state_op_gvlog gl in
 
   (* sequence ordered by time of each log entry *)
-  let itsl = time_seq_idx gl in
-  lemma_partition_idx_seq_interleaving itsl;
-  let tsl = project_seq itsl in
-  //assert(interleave tsl gl);
-  assume(interleave tsl gl);
+  let itsl = TL.create gl in  
+  lemma_interleaving_correct itsl;
+  assert(interleave (i_seq itsl) gl);
 
   (* sequence of state ops induced by tmsl *)
-  let tm_ops = to_state_op_vlog tsl in
+  let ts_ops = state_ops itsl in
 
-  lemma_vlog_interleave_implies_state_ops_interleave tsl gl;
-  assert(interleave tm_ops g_ops);
+  lemma_vlog_interleave_implies_state_ops_interleave (i_seq itsl) gl;
+  assert(interleave ts_ops g_ops);
 
   (* if tm_ops is read-write consistent then we have a contradiction *)
-  let is_rw_consistent = valid_all_comp ssm tm_ops in
-
+  let is_rw_consistent = valid_all_comp ssm ts_ops in
+  lemma_state_sm_equiv_rw_consistent ts_ops;
+  
   if is_rw_consistent then (
-
-    assert(valid_all ssm tm_ops);
-    lemma_state_sm_equiv_rw_consistent tm_ops;
-    assert(rw_consistent tm_ops);
+    assert(valid_all ssm ts_ops);
+    assert(rw_consistent ts_ops);
 
     (* a contradiction *)
     assert(seq_consistent g_ops);
@@ -100,6 +87,8 @@ let lemma_verifier_correct (gl: VG.hash_verifiable_log { ~ (seq_consistent (to_s
     (* any return value *)
     SingleHashCollision (Collision (DVal Null) (DVal Null))
   )
-  else
+  else  
+    //assert(~ (rw_consistent ts_ops));
     lemma_time_seq_rw_consistent itsl
   
+
