Veritas.Verifier.Merkle.fsti
@@ -9,6 +9,7 @@ open Veritas.SeqAux
 open Veritas.Verifier
 open Veritas.Verifier.TSLog
 
+module I = Veritas.Interleave
 module V = Veritas.Verifier
 module TL = Veritas.Verifier.TSLog
 
@@ -30,15 +31,15 @@ let mv_points_to (v:merkle_value) (d:bin_tree_dir) (k:key): bool =
 let mv_evicted_to_blum (v:merkle_value) (d:bin_tree_dir {mv_points_to_some v d}): bool =
   Desc?.b (desc_hash_dir v d)
 
-let eac_merkle_value (#p:pos) (itsl: eac_ts_log p) (k:merkle_key): merkle_value =
+let eac_merkle_value (itsl: TL.eac_log) (k:merkle_key): merkle_value =
   to_merkle_value (eac_value itsl k)
 
 (* the ancestor who holds the proof of the value of key k *)
-val proving_ancestor (#p:pos) (itsl: eac_ts_log p) (k:key{k <> Root}):
+val proving_ancestor (itsl: TL.eac_log) (k:key{k <> Root}):
   k':key{is_proper_desc k k'}
 
 (* after the first add the proving ancestor always points to self *)
-val lemma_proving_ancestor_points_to_self (#p:pos) (itsl: eac_ts_log p) (k:key{k <> Root}):
+val lemma_proving_ancestor_points_to_self (itsl: TL.eac_log) (k:key{k <> Root}):
   Lemma (requires not (is_eac_state_init itsl k))
         (ensures (mv_points_to (eac_merkle_value itsl (proving_ancestor itsl k))
                                (desc_dir k (proving_ancestor itsl k))
@@ -46,7 +47,7 @@ val lemma_proving_ancestor_points_to_self (#p:pos) (itsl: eac_ts_log p) (k:key{k
         [SMTPat (proving_ancestor itsl k)]
 
 (* before the first add the proving ancestor points to none or to a key that is not an ancestor *)
-val lemma_proving_ancestor_initial (#p:pos) (itsl: eac_ts_log p) (k:key{k <> Root}):
+val lemma_proving_ancestor_initial (itsl: TL.eac_log) (k:key{k <> Root}):
   Lemma (requires (is_eac_state_init itsl k))
         (ensures (mv_points_to_none (eac_merkle_value itsl (proving_ancestor itsl k))
                                     (desc_dir k (proving_ancestor itsl k)) \/
@@ -55,7 +56,7 @@ val lemma_proving_ancestor_initial (#p:pos) (itsl: eac_ts_log p) (k:key{k <> Roo
 
 (* if the proving ancestor of k is not Root, then Root points to some proper ancestor of 
  * k along that direction *)
-val lemma_non_proving_ancestor_root (#p:pos) (itsl: eac_ts_log p) (k:key{k <> Root}):
+val lemma_non_proving_ancestor_root (itsl: TL.eac_log) (k:key{k <> Root}):
   Lemma (requires (Root <> proving_ancestor itsl k))
         (ensures (is_proper_desc k Root /\
                   mv_points_to_some (eac_merkle_value itsl Root)
@@ -64,7 +65,7 @@ val lemma_non_proving_ancestor_root (#p:pos) (itsl: eac_ts_log p) (k:key{k <> Ro
                                                    (desc_dir k Root))))
 
 (* version of the previous lemma for non-root keys *)
-val lemma_non_proving_ancestor (#p:pos) (itsl: eac_ts_log p) (k:key{k <> Root}) (k':key{is_proper_desc k k'}):
+val lemma_non_proving_ancestor (itsl: TL.eac_log) (k:key{k <> Root}) (k':key{is_proper_desc k k'}):
   Lemma (requires (k' <> proving_ancestor itsl k) /\ not (is_eac_state_init itsl k))
         (ensures (mv_points_to_some (eac_merkle_value itsl k')
                                     (desc_dir k k')) /\
@@ -72,32 +73,32 @@ val lemma_non_proving_ancestor (#p:pos) (itsl: eac_ts_log p) (k:key{k <> Root}) 
                                                    (desc_dir k k'))))
 
 (* when evicted as merkle the proving ancestor contains our hash *)
-val lemma_proving_ancestor_has_hash (#p:pos) (itsl: eac_ts_log p) (k:key{k<> Root}):
+val lemma_proving_ancestor_has_hash (itsl: TL.eac_log) (k:key{k<> Root}):
   Lemma (requires (is_eac_state_evicted_merkle itsl k))
         (ensures (mv_pointed_hash (eac_merkle_value itsl (proving_ancestor itsl k))
                                   (desc_dir k (proving_ancestor itsl k)) = 
                   hashfn (eac_value itsl k)))
 
 (* when evicted as blum the proving ancestor contains a bit indicating the eviction *)
-val lemma_proving_ancestor_blum_bit (#p:pos) (itsl: eac_ts_log p) (k:key{k <> Root}):
+val lemma_proving_ancestor_blum_bit (itsl: TL.eac_log) (k:key{k <> Root}):
   Lemma (requires (is_eac_state_evicted itsl k))
         (ensures (mv_evicted_to_blum (eac_merkle_value itsl (proving_ancestor itsl k))
                                      (desc_dir k (proving_ancestor itsl k)) = 
                   is_eac_state_evicted_blum itsl k))
       
-val lemma_addm_ancestor_is_proving (#p:pos) (itsl: its_log p {length itsl > 0}):
-  Lemma (requires (TL.is_eac_log (prefix itsl (length itsl - 1)) /\
-                   AddM? (its_vlog_entry itsl (length itsl - 1))))
-        (ensures (Root <> V.key_of (its_vlog_entry itsl (length itsl - 1)) /\        
-                  AddM?.k' (its_vlog_entry itsl (length itsl - 1)) = 
-                  proving_ancestor (prefix itsl (length itsl - 1))
-                                   (V.key_of (its_vlog_entry itsl (length itsl - 1)))))
+val lemma_addm_ancestor_is_proving (itsl: its_log {I.length itsl > 0}):
+  Lemma (requires (TL.is_eac (I.prefix itsl (I.length itsl - 1)) /\
+                   AddM? (I.index itsl (I.length itsl - 1))))
+        (ensures (Root <> V.key_of (I.index itsl (I.length itsl - 1)) /\        
+                  AddM?.k' (I.index itsl (I.length itsl - 1)) = 
+                  proving_ancestor (I.prefix itsl (I.length itsl - 1))
+                                   (V.key_of (I.index itsl (I.length itsl - 1)))))
 
 (* if the store contains a k, it contains its proving ancestor *)
-val lemma_store_contains_proving_ancestor (#p:pos) (itsl: eac_ts_log p) 
-  (tid:nat{tid < p}) (k:key{k <> Root}):
-  Lemma (store_contains (thread_store (verifier_thread_state itsl tid)) k ==>
-         store_contains (thread_store (verifier_thread_state itsl tid)) 
+val lemma_store_contains_proving_ancestor (itsl: TL.eac_log) 
+  (tid:TL.valid_tid itsl) (k:key{k <> Root}):
+  Lemma (store_contains (TL.thread_store itsl tid) k ==>
+         store_contains (TL.thread_store itsl tid)
                         (proving_ancestor itsl k))
 
 
